theories/examples/enclaves/mutual_attestation_spec.v
@@ -10,9 +10,10 @@ From cap_machine Require Import
 
 
 Section mutual_attest_main.
-  Context {Σ:gFunctors} {ceriseg:ceriseG Σ} {sealsg : sealStoreG Σ}
-    `{reservedaddresses : ReservedAddresses}
-    {nainv: logrel_na_invs Σ} `{MP: MachineParameters}.
+  Context {Σ:gFunctors} {ceriseg:ceriseG Σ} {sealsg: sealStoreG Σ}
+          {nainv: logrel_na_invs Σ}
+          {reservedaddresses : ReservedAddresses}
+          `{MP: MachineParameters}.
   Context {MA: MutualAttestation}.
 
 
@@ -21,18 +22,14 @@ Section mutual_attest_main.
   (* -------------------------------------------------- *)
 
   Lemma mutual_attest_contract :
-    custom_enclave_contract ma_enclaves_map.
+    ⊢ custom_enclave_contract (enclaves_map := contract_ma_enclaves_map).
   Proof.
-    rewrite /custom_enclave_contract.
+    iLöb as "IH".
+    iEval (rewrite /custom_enclave_contract).
     iIntros (I b e a v b' e' a' v' enclave_data ot ce
-      Hwf_cemap Hcode_ce Hot Hb' HIhash Hb He)
+      Hcode_ce Hot Hb' HIhash Hb He)
       "(#Henclaves_inv & #Hma_inv & #HPenc & #HPsign)".
-    clear HIhash.
-    clear Hwf_cemap.
     assert (e = (b ^+ (length (code ce) + 1))%a) as -> by solve_addr+He.
-
-    rewrite /ma_enclaves_map in Hcode_ce.
-    simplify_map_eq.
 
     assert (I = hash_mutual_attest_A \/ I = hash_mutual_attest_B) as HI.
     { rewrite lookup_insert_Some in Hcode_ce.
@@ -41,18 +38,23 @@ Section mutual_attest_main.
       destruct Hcode_ce as [ [? _] | [_ Hcode_ce] ]; first auto.
       done.
     }
-    destruct HI ; simplify_map_eq.
-    - iApply ( mutual_attest_A_contract with "[]") ; last iFrame "#"; eauto.
+    destruct HI.
+		- rewrite H in HIhash.
+			simplify_map_eq.
+			rewrite /ma_enclaves_map lookup_insert // in Hcode_ce; simplify_eq.
+			iApply ( mutual_attest_A_contract with "[]") ; last iFrame "#"; eauto.
     - rewrite lookup_insert_ne // in Hcode_ce.
-      2:{ rewrite /hash_mutual_attest_A /hash_mutual_attest_B.
-          intro Hcontra.
+      2:{
+        rewrite H.
+        rewrite /hash_mutual_attest_A /hash_mutual_attest_B.
+        intro Hcontra.
           apply hash_concat_inj' in Hcontra.
           destruct Hcontra as [_ Hcontra].
-          rewrite /mutual_attest_enclave_A_code /mutual_attest_enclave_B_code in Hcontra.
           by injection Hcontra.
       }
       simplify_map_eq.
       iApply ( mutual_attest_B_contract with "[]") ; last iFrame "#"; eauto.
+      by rewrite H0.
   Qed.
 
   (* -------------------------------------------------- *)
@@ -77,14 +79,13 @@ Section mutual_attest_main.
     ( PC ↦ᵣ LCap RX pc_b pc_e pc_a pc_v
       ∗ r ↦ᵣ w ∗ r_t5 ↦ᵣ w5 ∗ r_t6 ↦ᵣ w6
       ∗ codefrag pc_a pc_v code
-      ∗ custom_enclave_inv ma_enclaves_map
+      ∗ custom_enclave_inv (enclaves_map := contract_ma_enclaves_map)
       ∗ ▷ ( (∃ tid ECn,
                 ⌜ has_seal otype_w tid ⌝
                 ∗ ⌜ 0 <= tid < ECn ⌝
                 ∗ (
                     □ ∀ (I : EIdentity) (tid : TIndex) (ot : OType) (ce : CustomEnclave),
                       (⌜(0 <= tid < ECn)⌝) -∗
-                      (⌜ @custom_enclaves_map_wf Σ _ ma_enclaves_map ⌝) -∗
                       enclave_all tid I
                       ∗ ⌜ ma_enclaves_map !! I = Some ce ⌝
                       ∗ ⌜ has_seal ot tid ⌝ -∗
@@ -167,7 +168,6 @@ Section mutual_attest_main.
       ∗ (
           □ ∀ (I : EIdentity) (tid : TIndex) (ot : OType) (ce : CustomEnclave),
             (⌜(0 <= tid < ECn)⌝) -∗
-            (⌜ @custom_enclaves_map_wf Σ _ ma_enclaves_map ⌝) -∗
             enclave_all tid I
             ∗ ⌜ ma_enclaves_map !! I = Some ce ⌝
             ∗ ⌜ has_seal ot tid ⌝ -∗
@@ -225,11 +225,7 @@ Section mutual_attest_main.
         else seal_pred (a ^+ -1)%f (Penc mutual_attest_enclave_pred)
              ∗ seal_pred a (Psign mutual_attest_enclave_pred)
       )%I as "Hma".
-    {
-      iApply "Hcemap"; iFrame "%#∗".
-      iPureIntro. rewrite /ma_enclaves_map.
-      by apply wf_ma_enclaves_map.
-    }
+    { iApply "Hcemap"; iFrame "%#∗". }
     rewrite HPenc.
     destruct (Z.even (finz.to_z a)) eqn:HEven_a
     ; iDestruct "Hma" as "[Hma_Penc Hma_Psign]"
@@ -374,7 +370,7 @@ Section mutual_attest_main.
     (link_table_inv v_link assert_entry b_assert e_assert v_assert
     ∗ assert_inv b_assert a_flag e_assert v_assert
     ∗ flag_inv a_flag v_assert)
-    ∗ custom_enclave_inv ma_enclaves_map
+		∗ custom_enclave_inv (enclaves_map := contract_ma_enclaves_map)
     ∗ full_map rmap
     ∗ (∀ (r : RegName) (lv : LWord), ⌜r ≠ PC⌝ → ⌜rmap !! r = Some lv⌝ → fixpoint interp1 lv)
 
