theories/ftlr/EInit.v
@@ -10,8 +10,7 @@ Section fundamental.
           {nainv: logrel_na_invs Σ}
           {reservedaddresses : ReservedAddresses}
           `{MP: MachineParameters}
-          {contract_enclaves : CustomEnclavesMap}
-  .
+          {contract_enclaves : @CustomEnclavesMap Σ MP}.
 
   Notation D := ((leibnizO LWord) -n> iPropO Σ).
   Notation R := ((leibnizO LReg) -n> iPropO Σ).
@@ -38,7 +37,7 @@ Section fundamental.
     ftlr_instr lregs p_pc b_pc e_pc a_pc v_pc lw_pc (EInit src) P.
   Proof.
     intros Hp Hsome i Hbae Hi.
-    iIntros "#HsysInv #IH #Hinv #Hinva #Hreg #(Hread & Hwrite & %HpersP) Hown Ha HP Hcls HPC Hmap".
+    iIntros "[Hcontract #Hsystem_inv] #IH #Hinv #Hinva #Hreg #(Hread & Hwrite & %HpersP) Hown Ha HP Hcls HPC Hmap".
     specialize (HpersP lw_pc).
     rewrite delete_insert_delete.
     iDestruct ((big_sepM_delete _ _ PC) with "[HPC Hmap]") as "Hmap /=";
@@ -932,141 +931,141 @@ Section fundamental.
     (* } *)
 
 
-  Lemma einit_case (lregs : leibnizO LReg)
-    (p_pc : Perm) (b_pc e_pc a_pc : Addr) (v_pc : Version)
-    (lw_pc : LWord) (src : RegName) (P : D):
-    ftlr_instr lregs p_pc b_pc e_pc a_pc v_pc lw_pc (EInit src) P.
-  Proof.
-    intros Hp Hsome HcorrectLPC Hbae Hi.
-    iIntros "#IH #Hinv #Hinva #Hreg #(Hread & Hwrite & %HpersP) Hown Ha #HP Hcls HPC Hmap".
-    specialize (HpersP lw_pc).
-    rewrite delete_insert_delete.
-    iDestruct ((big_sepM_delete _ _ PC) with "[HPC Hmap]") as "Hmap /=";
-      [apply lookup_insert|rewrite delete_insert_delete;iFrame|]. simpl.
+  (* Lemma einit_case (lregs : leibnizO LReg) *)
+  (*   (p_pc : Perm) (b_pc e_pc a_pc : Addr) (v_pc : Version) *)
+  (*   (lw_pc : LWord) (src : RegName) (P : D): *)
+  (*   ftlr_instr lregs p_pc b_pc e_pc a_pc v_pc lw_pc (EInit src) P. *)
+  (* Proof. *)
+  (*   intros Hp Hsome HcorrectLPC Hbae Hi. *)
+  (*   iIntros "#IH #Hinv #Hinva #Hreg #(Hread & Hwrite & %HpersP) Hown Ha #HP Hcls HPC Hmap". *)
+  (*   specialize (HpersP lw_pc). *)
+  (*   rewrite delete_insert_delete. *)
+  (*   iDestruct ((big_sepM_delete _ _ PC) with "[HPC Hmap]") as "Hmap /="; *)
+  (*     [apply lookup_insert|rewrite delete_insert_delete;iFrame|]. simpl. *)
 
-    (* To read out PC's name later, and needed when calling wp_load *)
-    assert(∀ x : RegName, is_Some (<[PC:=LCap p_pc b_pc e_pc a_pc v_pc]> lregs !! x)) as Hsome'.
-    {
-      intros. destruct (decide (x = PC)) as [Hx|Hx].
-      rewrite Hx lookup_insert; unfold is_Some. by eexists.
-      by rewrite lookup_insert_ne.
-    }
+  (*   (* To read out PC's name later, and needed when calling wp_load *) *)
+  (*   assert(∀ x : RegName, is_Some (<[PC:=LCap p_pc b_pc e_pc a_pc v_pc]> lregs !! x)) as Hsome'. *)
+  (*   { *)
+  (*     intros. destruct (decide (x = PC)) as [Hx|Hx]. *)
+  (*     rewrite Hx lookup_insert; unfold is_Some. by eexists. *)
+  (*     by rewrite lookup_insert_ne. *)
+  (*   } *)
 
-    (* Initializing the names for the values of Hsrc now, to instantiate the existentials in step 1 *)
-    assert (∃ p_src b_src e_src a_src v_src, read_reg_inr (<[PC:=LCap p_pc b_pc e_pc a_pc v_pc]> lregs) src p_src b_src e_src a_src v_src)
-      as (p_src & b_src & e_src & a_src & v_src & HV_Src).
-    {
-      specialize Hsome' with src as Hsrc.
-      destruct Hsrc as [wsrc Hsome_src].
-      unfold read_reg_inr. rewrite Hsome_src.
-      destruct wsrc as [|[ p_src b_src e_src a_src v_src|] | ]; try done.
-      by repeat eexists.
-    }
+  (*   (* Initializing the names for the values of Hsrc now, to instantiate the existentials in step 1 *) *)
+  (*   assert (∃ p_src b_src e_src a_src v_src, read_reg_inr (<[PC:=LCap p_pc b_pc e_pc a_pc v_pc]> lregs) src p_src b_src e_src a_src v_src) *)
+  (*     as (p_src & b_src & e_src & a_src & v_src & HV_Src). *)
+  (*   { *)
+  (*     specialize Hsome' with src as Hsrc. *)
+  (*     destruct Hsrc as [wsrc Hsome_src]. *)
+  (*     unfold read_reg_inr. rewrite Hsome_src. *)
+  (*     destruct wsrc as [|[ p_src b_src e_src a_src v_src|] | ]; try done. *)
+  (*     by repeat eexists. *)
+  (*   } *)
 
-    (* Step 1: prepare all resources necessary to open the invariants of the argument (the cap given in is_unique), if necessary,
-       and store all the resources obtained from the region in allow_load_res *)
-    iDestruct (create_einit_code_resources with "[$Hreg] [$Hinv]") as (Ps_code) "[%Hlen_Ps HEinitCodeRes]"
-    ; [ eassumption
-      | by apply elem_of_finz_seq_between
-      |].
+  (*   (* Step 1: prepare all resources necessary to open the invariants of the argument (the cap given in is_unique), if necessary, *)
+  (*      and store all the resources obtained from the region in allow_load_res *) *)
+  (*   iDestruct (create_einit_code_resources with "[$Hreg] [$Hinv]") as (Ps_code) "[%Hlen_Ps HEinitCodeRes]" *)
+  (*   ; [ eassumption *)
+  (*     | by apply elem_of_finz_seq_between *)
+  (*     |]. *)
 
-    (* Open the invariants! *)
-    (* Step 2: derive the concrete map of memory we need, and any spatial predicates holding over it *)
-    iMod (einit_code_resources_implies_mem_map with "HEinitCodeRes Ha") as (lmem) "[HEinitCodeMem HMemCodeRes]".
-    (* rename the big masks to easy names *)
-    set (E0 := ⊤ ∖ ↑logN.@(a_pc, v_pc)).
-    set (E1 := allow_einit_code_mask a_pc v_pc (code_addresses a_pc (finz.seq_between b_src e_src)) v_src).
+  (*   (* Open the invariants! *) *)
+  (*   (* Step 2: derive the concrete map of memory we need, and any spatial predicates holding over it *) *)
+  (*   iMod (einit_code_resources_implies_mem_map with "HEinitCodeRes Ha") as (lmem) "[HEinitCodeMem HMemCodeRes]". *)
+  (*   (* rename the big masks to easy names *) *)
+  (*   set (E0 := ⊤ ∖ ↑logN.@(a_pc, v_pc)). *)
+  (*   set (E1 := allow_einit_code_mask a_pc v_pc (code_addresses a_pc (finz.seq_between b_src e_src)) v_src). *)
 
-    (* Step 3:  derive the non-spatial conditions over the memory map*)
-    iDestruct (mem_map_implies_pure_conds with "HEinitCodeMem") as %HReadPC.
+  (*   (* Step 3:  derive the non-spatial conditions over the memory map*) *)
+  (*   iDestruct (mem_map_implies_pure_conds with "HEinitCodeMem") as %HReadPC. *)
 
-    (* Step 4: move the later outside, so that we can remove it after applying wp_isunique *)
-    (* iDestruct (allow_einit_code_mem_later with "HSweepMem") as "HSweepMem"; auto. *)
+  (*   (* Step 4: move the later outside, so that we can remove it after applying wp_isunique *) *)
+  (*   (* iDestruct (allow_einit_code_mem_later with "HSweepMem") as "HSweepMem"; auto. *) *)
 
-    iAssert ( ⌜ allows_einit_code (<[PC:=LCap p_pc b_pc e_pc a_pc v_pc]> lregs) src ⌝)%I as "%Hallows_einit_code".
-    { iDestruct "HEinitCodeRes" as "(_&%HeinitCodeRes&_)".
-      iPureIntro. apply HeinitCodeRes.
-    }
+  (*   iAssert ( ⌜ allows_einit_code (<[PC:=LCap p_pc b_pc e_pc a_pc v_pc]> lregs) src ⌝)%I as "%Hallows_einit_code". *)
+  (*   { iDestruct "HEinitCodeRes" as "(_&%HeinitCodeRes&_)". *)
+  (*     iPureIntro. apply HeinitCodeRes. *)
+  (*   } *)
 
-    (* iAssert ( ⌜ *)
-    (*             if ( einit_code_mask_cond (<[PC:=LCap p_pc b_pc e_pc a_pc v_pc]> lregs) src p_src b_src e_src a_src v_src a_pc v_pc ) *)
-    (*             then (∃ dcap, lmem !! (b_src, v_src) = Some dcap) *)
-    (*             else True ⌝ )%I as "%Hdcap". *)
-    (* { admit. } *)
+  (*   (* iAssert ( ⌜ *) *)
+  (*   (*             if ( einit_code_mask_cond (<[PC:=LCap p_pc b_pc e_pc a_pc v_pc]> lregs) src p_src b_src e_src a_src v_src a_pc v_pc ) *) *)
+  (*   (*             then (∃ dcap, lmem !! (b_src, v_src) = Some dcap) *) *)
+  (*   (*             else True ⌝ )%I as "%Hdcap". *) *)
+  (*   (* { admit. } *) *)
 
 
-    Set Nested Proofs Allowed.
-    Fixpoint list_remove_elem_list `{A : Type} `{EqDecision A} (la' la : list A) : list A :=
-      match la' with
-      | [] => la
-      | h::t => list_remove_elem h (list_remove_elem_list t la)
-      end.
+  (*   Set Nested Proofs Allowed. *)
+  (*   Fixpoint list_remove_elem_list `{A : Type} `{EqDecision A} (la' la : list A) : list A := *)
+  (*     match la' with *)
+  (*     | [] => la *)
+  (*     | h::t => list_remove_elem h (list_remove_elem_list t la) *)
+  (*     end. *)
 
-    Definition data_addresses (a_pc : Addr) (la_code la_data : list Addr)
-      := (list_remove_elem_list (a_pc::la_code) la_data).
+  (*   Definition data_addresses (a_pc : Addr) (la_code la_data : list Addr) *)
+  (*     := (list_remove_elem_list (a_pc::la_code) la_data). *)
 
-    Definition allow_einit_data_mask
-      (a_pc : Addr) (v_pc : Version)
-      (la_code : list Addr) (v_code : Version)
-      (la_data : list Addr) (v_data : Version)
-      : coPset :=
-      let mask_code := allow_einit_code_mask a_pc v_pc la_code v_code in
-      compute_mask_region mask_code (data_addresses a_pc la_code la_data) v_data.
+  (*   Definition allow_einit_data_mask *)
+  (*     (a_pc : Addr) (v_pc : Version) *)
+  (*     (la_code : list Addr) (v_code : Version) *)
+  (*     (la_data : list Addr) (v_data : Version) *)
+  (*     : coPset := *)
+  (*     let mask_code := allow_einit_code_mask a_pc v_pc la_code v_code in *)
+  (*     compute_mask_region mask_code (data_addresses a_pc la_code la_data) v_data. *)
 
-  Definition read_lmem_inr (lmem : LMem) (a : Addr) (v : Version) p' b' e' a' v' :=
-    match lmem !! (a,v) with
-      | Some (LCap p'' b'' e'' a'' v'') => (LCap p'' b'' e'' a'' v'') = LCap p' b' e' a' v'
-      | Some _ => True
-      | None => False end.
+  (* Definition read_lmem_inr (lmem : LMem) (a : Addr) (v : Version) p' b' e' a' v' := *)
+  (*   match lmem !! (a,v) with *)
+  (*     | Some (LCap p'' b'' e'' a'' v'') => (LCap p'' b'' e'' a'' v'') = LCap p' b' e' a' v' *)
+  (*     | Some _ => True *)
+  (*     | None => False end. *)
 
-  Definition mem_allows_einit_data
-    (lmem : LMem) (a : Addr) (v : Version)
-    (p' : Perm) (b' e' a' : Addr) (v' : Version):=
-    lmem !! (a,v) = Some (LCap p' b' e' a' v') ∧ p' = RW.
+  (* Definition mem_allows_einit_data *)
+  (*   (lmem : LMem) (a : Addr) (v : Version) *)
+  (*   (p' : Perm) (b' e' a' : Addr) (v' : Version):= *)
+  (*   lmem !! (a,v) = Some (LCap p' b' e' a' v') ∧ p' = RW. *)
 
-  Definition einit_data_mask_cond
-    (lmem : LMem) (b_code : Addr) (v_code : Version)
-    (p_data : Perm) (b_data e_data a_data : Addr) (v_data : Version)
-    (a_pc : Addr) (v_pc : Version) :=
-    decide (
-        mem_allows_einit_data lmem b_code v_code p_data b_data e_data a_data v_data
-        ∧ a_pc ∉ (finz.seq_between b_data e_data)
-      ).
+  (* Definition einit_data_mask_cond *)
+  (*   (lmem : LMem) (b_code : Addr) (v_code : Version) *)
+  (*   (p_data : Perm) (b_data e_data a_data : Addr) (v_data : Version) *)
+  (*   (a_pc : Addr) (v_pc : Version) := *)
+  (*   decide ( *)
+  (*       mem_allows_einit_data lmem b_code v_code p_data b_data e_data a_data v_data *)
+  (*       ∧ a_pc ∉ (finz.seq_between b_data e_data) *)
+  (*     ). *)
 
-  Definition interp_list_pred_data
-    (lws : list LWord) (Ps : list D) (has_later : bool) : iProp Σ :=
-    ([∗ list] lw;Pw ∈ lws;Ps, (if has_later then ▷▷ (Pw : D) lw else (Pw : D) lw)).
+  (* Definition interp_list_pred_data *)
+  (*   (lws : list LWord) (Ps : list D) (has_later : bool) : iProp Σ := *)
+  (*   ([∗ list] lw;Pw ∈ lws;Ps, (if has_later then ▷▷ (Pw : D) lw else (Pw : D) lw)). *)
 
-  Definition interp_list_persistent_data
-    (lws : list LWord) (Ps : list D) : iProp Σ :=
-    ( ⌜ Persistent ([∗ list] lw;Pw ∈ lws;Ps, (Pw : D) lw) ⌝ ).
+  (* Definition interp_list_persistent_data *)
+  (*   (lws : list LWord) (Ps : list D) : iProp Σ := *)
+  (*   ( ⌜ Persistent ([∗ list] lw;Pw ∈ lws;Ps, (Pw : D) lw) ⌝ ). *)
 
-  Definition interp_list_readcond_data
-    (lws : list LWord) (Ps : list D) (has_later : bool) : iProp Σ :=
-    ( if has_later
-      then [∗ list] Pa ∈ Ps, ▷ read_cond Pa interp
-      else [∗ list] Pa ∈ Ps, (□ ∀ (lw : LWord), (Pa : D) lw -∗ interp lw)
-    )%I.
+  (* Definition interp_list_readcond_data *)
+  (*   (lws : list LWord) (Ps : list D) (has_later : bool) : iProp Σ := *)
+  (*   ( if has_later *)
+  (*     then [∗ list] Pa ∈ Ps, ▷ read_cond Pa interp *)
+  (*     else [∗ list] Pa ∈ Ps, (□ ∀ (lw : LWord), (Pa : D) lw -∗ interp lw) *)
+  (*   )%I. *)
 
-  Definition interp_list_close_data
-    (la : list Addr) (Ps : list D) (v : Version) (E E' : coPset) : iProp Σ :=
-    ( ▷ (▷ ([∗ list] a_Pa ∈ zip la Ps, (interp_ref_inv a_Pa.1 v a_Pa.2))) ={E', E }=∗ True).
+  (* Definition interp_list_close_data *)
+  (*   (la : list Addr) (Ps : list D) (v : Version) (E E' : coPset) : iProp Σ := *)
+  (*   ( ▷ (▷ ([∗ list] a_Pa ∈ zip la Ps, (interp_ref_inv a_Pa.1 v a_Pa.2))) ={E', E }=∗ True). *)
 
-  Definition resources_open_invariant_data
-    (a_pc : Addr) (v_pc : Version)
-    (la_code : list Addr) (v_code : Version)
-    (la_data : list Addr) (v_data : Version) (lws_data : list LWord) (Ps_data : list D)
-    (has_later : bool)
-    : iProp Σ :=
+  (* Definition resources_open_invariant_data *)
+  (*   (a_pc : Addr) (v_pc : Version) *)
+  (*   (la_code : list Addr) (v_code : Version) *)
+  (*   (la_data : list Addr) (v_data : Version) (lws_data : list LWord) (Ps_data : list D) *)
+  (*   (has_later : bool) *)
+  (*   : iProp Σ := *)
 
-    (* let E0 := ⊤ ∖ ↑logN.@(a_pc, v_pc) in *)
-    let E1 := allow_einit_code_mask a_pc v_pc la_code v_code : coPset in
-    let E2 := allow_einit_data_mask a_pc v_pc la_code v_code la_data v_data : coPset in
+  (*   (* let E0 := ⊤ ∖ ↑logN.@(a_pc, v_pc) in *) *)
+  (*   let E1 := allow_einit_code_mask a_pc v_pc la_code v_code : coPset in *)
+  (*   let E2 := allow_einit_data_mask a_pc v_pc la_code v_code la_data v_data : coPset in *)
 
-    interp_list_pred_data lws_data Ps_data has_later
-    ∗ interp_list_persistent_data lws_data Ps_data
-    ∗ interp_list_readcond_data lws_data Ps_data has_later
-    ∗ interp_list_close_data la_data Ps_data v_data E1 E2.
+  (*   interp_list_pred_data lws_data Ps_data has_later *)
+  (*   ∗ interp_list_persistent_data lws_data Ps_data *)
+  (*   ∗ interp_list_readcond_data lws_data Ps_data has_later *)
+  (*   ∗ interp_list_close_data la_data Ps_data v_data E1 E2. *)
 
 
   (* Definition allow_einit_data_resources *)
@@ -1143,10 +1142,10 @@ Section fundamental.
     (* Admitted. *)
 
     (* Initializing the names for the values of Hsrc now, to instantiate the existentials in step 1 *)
-    assert (∃ p_data b_data e_data a_data v_data,
-               read_lmem_inr lmem b_src v_src  p_data b_data e_data a_data v_data)
-      as (p_data & b_data & e_data & a_data & v_data & HV_data).
-    { admit. }
+    (* assert (∃ p_data b_data e_data a_data v_data, *)
+    (*            read_lmem_inr lmem b_src v_src  p_data b_data e_data a_data v_data) *)
+    (*   as (p_data & b_data & e_data & a_data & v_data & HV_data). *)
+    (* { admit. } *)
 
     (* iDestruct (create_einit_data_resources with "[$HEinitCodeRes] [$HEinitCodeMem] [$HMemCodeRes]") *)
     (*   as (Ps_data) "(%Hlen_Ps_data & _ & HEinitCodeMem & Hmem & HEinitDataRes)"; first eassumption. *)
@@ -1232,7 +1231,7 @@ Section fundamental.
   (*       eauto *)
   (*     | | | ]. *)
 
-  Admitted.
+  (* Admitted. *)
 
 
 
