theories/ftlr/EStoreId.v
@@ -10,8 +10,7 @@ Section fundamental.
           {nainv: logrel_na_invs Σ}
           {reservedaddresses : ReservedAddresses}
           `{MP: MachineParameters}
-          {contract_enclaves : CustomEnclavesMap}
-  .
+          {contract_enclaves : @CustomEnclavesMap Σ MP}.
 
   Notation D := ((leibnizO LWord) -n> iPropO Σ).
   Notation R := ((leibnizO LReg) -n> iPropO Σ).
@@ -24,7 +23,7 @@ Section fundamental.
     ftlr_instr lregs p b e a v lw (EStoreId rd rs) P.
   Proof.
     intros Hp Hsome i Hbae Hi.
-    iIntros "#HsysInv #IH #Hinv #Hinva #Hreg #Hread Hown Ha HP Hcls HPC Hmap".
+    iIntros "[Hcontract #Hsystem_inv] #IH #Hinv #Hinva #Hreg #Hread Hown Ha HP Hcls HPC Hmap".
     rewrite delete_insert_delete.
     specialize Hsome with rd as Hrd.
     specialize Hsome with rs as Hrs.
