theories/ftlr/IsUnique.v
@@ -11,8 +11,7 @@ Section fundamental.
           {nainv: logrel_na_invs Σ}
           {reservedaddresses : ReservedAddresses}
           `{MP: MachineParameters}
-          {contract_enclaves : CustomEnclavesMap}
-  .
+          {contract_enclaves : @CustomEnclavesMap Σ MP}.
 
   Notation D := ((leibnizO LWord) -n> iPropO Σ).
   Notation R := ((leibnizO LReg) -n> iPropO Σ).
@@ -716,7 +715,7 @@ Section fundamental.
     ftlr_instr lregs p_pc b_pc e_pc a_pc v_pc lw_pc (IsUnique dst src) P.
   Proof.
     intros Hp Hsome HcorrectLPC Hbae Hi.
-    iIntros "#HsysInv #IH #Hinv #Hinva #Hreg #(Hread & Hwrite & %HpersP) Hown Ha #HP Hcls HPC Hmap".
+    iIntros "[Hcontract #Hsystem_inv] #IH #Hinv #Hinva #Hreg #(Hread & Hwrite & %HpersP) Hown Ha #HP Hcls HPC Hmap".
     specialize (HpersP lw_pc).
     rewrite delete_insert_delete.
     iDestruct ((big_sepM_delete _ _ PC) with "[HPC Hmap]") as "Hmap /=";
